crypto/bignum/Hacl.Bignum.Fmul.fst
@@ -28,21 +28,24 @@ let shift_reduce output =
   shift output;
   reduce output
 
+
 #set-options "--z3rlimit 50 --initial_fuel 1 --max_fuel 1"
 
 val mul_shift_reduce_:
   output:felem_wide ->
+  init_input:Ghost.erased seqelem ->
   input:felem{disjoint output input} ->
   input2:felem{disjoint output input2 /\ disjoint input input2}  ->
   ctr:U32.t{U32.v ctr <= len} ->
   Stack unit
     (requires (fun h -> live h output /\ live h input /\ live h input2
-      /\ mul_shift_reduce_pre (as_seq h output) (as_seq h input) (as_seq h input2) (U32.v ctr)))
+      /\ mul_shift_reduce_pre (as_seq h output) (Ghost.reveal init_input) (as_seq h input) (as_seq h input2) (U32.v ctr)))
     (ensures (fun h0 _ h1 -> live h0 output /\ live h0 input /\ live h0 input2 /\ modifies_2 output input h0 h1
       /\ live h1 output /\ live h1 input
-      /\ mul_shift_reduce_pre (as_seq h0 output) (as_seq h0 input) (as_seq h0 input2) (U32.v ctr)
-      /\ as_seq h1 output == mul_shift_reduce_spec_ (as_seq h0 output) (Seq.create len limb_zero) (as_seq h0 input) (as_seq h0 input2) (U32.v ctr)))
-let rec mul_shift_reduce_ output input input2 ctr =
+      /\ mul_shift_reduce_pre (as_seq h0 output) (Ghost.reveal init_input) (as_seq h0 input) (as_seq h0 input2) (U32.v ctr)
+      /\ as_seq h1 output == mul_shift_reduce_spec_ (as_seq h0 output) (Ghost.reveal init_input) (as_seq h0 input) (as_seq h0 input2) (U32.v ctr)
+      ))
+let rec mul_shift_reduce_ output init_input input input2 ctr =
   let open FStar.UInt32 in
   if (ctr =^ 0ul) then ()
   else (
@@ -52,7 +55,7 @@ let rec mul_shift_reduce_ output input input2 ctr =
     let input2i = input2.(j) in
     sum_scalar_multiplication_ output input input2i clen;
     if (ctr >^ 1ul) then shift_reduce input;
-    mul_shift_reduce_ output input input2 i
+    mul_shift_reduce_ output init_input input input2 i
   )
 
 
@@ -75,7 +78,11 @@ let fmul_ output input input2 =
   let h1 = ST.get() in
   let t   = create wide_zero clen in
   let h2 = ST.get() in
-  mul_shift_reduce_ t input input2 clen;
+  (* TODO: something more developer friendly ? *)
+  let input_init = Ghost.elift2_p #HyperStack.mem #felem
+                                  #(fun h x -> live h x) #seqelem 
+                                  (as_seq) (Ghost.hide h2) (Ghost.hide input) in
+  mul_shift_reduce_ t input_init input input2 clen;
   carry_wide_ t 0ul;
   carry_top_wide t;
   copy_from_wide_ output t clen;
