crypto/bignum/Hacl.Bignum.Fmul.Spec2.fst
@@ -13,22 +13,21 @@ open Hacl.Bignum.Fmul.Spec
 
 module U32 = FStar.UInt32
 
+#set-options "--initial_fuel 0 --max_fuel 0"
 
-val fmul_spec: input:seqelem -> input2:seqelem{fmul_pre input input2} -> Tot (output:seqelem)
+val fmul_spec:
+  input:seqelem -> input2:seqelem{fmul_pre input input2} ->
+  Tot (output:seqelem{seval output % prime = (seval input * seval input2) % prime})
 let fmul_spec input input2 =
   lemma_mul_to_red input input2;
   let tmp = Seq.create len wide_zero in
   let output1 = mul_shift_reduce_spec input input2 in
   let output2 = carry_wide_spec output1 0 in
+  lemma_carry_top_wide_spec output2;
   let output3 = carry_top_wide_spec output2 in
+  lemma_copy_from_wide output3;
   let output4 = copy_from_wide_spec output3 in
   carry_0_to_1_spec output4
-
-
-val lemma_fmul_spec: input:seqelem -> input2:seqelem{fmul_pre input input2} -> Lemma
-  (seval (fmul_spec input input2) % prime = (seval input * seval input2) % prime)
-let lemma_fmul_spec input input2 =
-  admit() (* TOOD *)
 
 #set-options "--z3rlimit 40"
 
